

For part i) I referenced Essential Aspects of Bayesian Data Imputation by Holt and Nguyen
Holt, William, and Duy Nguyen. "Essential Aspects of Bayesian Data Imputation." Marist College, 2022.

2.5.i)

2.5 - 2.7 $x \sim \mathcal{N}(\bar{x}, P_{xx}), y \sim \mathcal{N}(\bar{y}, P_{yy})$

2.5i Let (x, y) be jointly Gaussian random vectors s.t.

$$\begin{pmatrix} x \\ y \end{pmatrix} \sim \mathcal{N}\left(\begin{pmatrix} \bar{x} \\ \bar{y} \end{pmatrix}, \begin{pmatrix} P_{xx} & P_{xy} \\ P_{yx} & P_{yy} \end{pmatrix}\right), P_{yy} > 0$$

i) show that $p(x|y) \sim \mathcal{N}(\hat{x}, P_{x|y})$

where $\hat{x} = \bar{x} + P_{xy}P_{yy}^{-1}(y - \bar{y})$ and $P_{x|y} = P_{xx} - P_{xy}P_{yy}^{-1}P_{yx}$

$$p(x|y) \sim \mathcal{N}(\bar{x} + P_{xy}P_{yy}^{-1}(y - \bar{y}), P_{xx} - P_{xy}P_{yy}^{-1}P_{yx})$$

$$\text{show } \mathbb{E}(p(x|y)) = \bar{x} + P_{xy}P_{yy}^{-1}(y - \bar{y}) = \hat{x}$$

$$= \mathbb{E}\left(\frac{P(x \cap y)}{P(y)}\right)$$

$$P_{xx} - P_{xy}P_{yy}^{-1}P_{yx} = \mathbb{E}((x - \hat{x})(x - \hat{x})^T) = P_{x|y}$$

$$\mathbb{E}(((x - \bar{x}) - P_{xy}P_{yy}^{-1}(y - \bar{y}))((x - \bar{x}) - P_{xy}P_{yy}^{-1}(y - \bar{y}))^T)$$

$$P_{xx} = \mathbb{E}((x - \bar{x})(x - \bar{x})^T)$$

$$\text{Proof: } p(x|y, \hat{x}, P_{x|y}) = \frac{1}{(2\pi)^{(d_1+d_2)/2} |P_{x|y}|^{1/2}} \exp\left(-\frac{1}{2} \begin{pmatrix} x - \bar{x} \\ y - \bar{y} \end{pmatrix}^T \begin{pmatrix} P_{xx} & P_{xy} \\ P_{yx} & P_{yy} \end{pmatrix}^{-1} \begin{pmatrix} x - \bar{x} \\ y - \bar{y} \end{pmatrix}\right)$$

Note the following identity is directly obtained

$$\begin{pmatrix} I & -P_{xy}P_{yy}^{-1} \\ 0 & I \end{pmatrix} \begin{pmatrix} P_{xx} & P_{xy} \\ P_{yx} & P_{yy} \end{pmatrix} \begin{pmatrix} I & 0 \\ -P_{yy}^{-1}P_{yx} & I \end{pmatrix} = \begin{pmatrix} P_{xx}/P_{yy} & 0 \\ 0 & P_{yy} \end{pmatrix} \quad (1)$$

⊙ Taking determinant of both sides of (1) we get

$$|P_{XY}| = \begin{vmatrix} P_{XX} & P_{XY} \\ P_{YX} & P_{YY} \end{vmatrix} = |P_{XY}/P_{YY}| |P_{YY}| \quad (2)$$

inverting both sides of (1)

$$\begin{pmatrix} P_{XX} & P_{XY} \\ P_{YX} & P_{YY} \end{pmatrix}^{-1} = \begin{pmatrix} I & 0 \\ -P_{YY}^{-1}P_{YX} & I \end{pmatrix} \begin{pmatrix} (P_{XY}/P_{YY})^{-1} & 0 \\ 0 & P_{YY}^{-1} \end{pmatrix} \begin{pmatrix} I & -P_{XX}P_{YY}^{-1} \\ 0 & I \end{pmatrix}$$

Resulting from this

$$\begin{aligned} p(x, y | \hat{x}, P_{XY}) &\propto \exp\left(-\frac{1}{2} \begin{pmatrix} x - \bar{x} \\ y - \bar{y} \end{pmatrix}^T \begin{pmatrix} P_{XX} & P_{XY} \\ P_{YX} & P_{YY} \end{pmatrix}^{-1} \begin{pmatrix} x - \bar{x} \\ y - \bar{y} \end{pmatrix}\right) \\ &= \exp\left(-\frac{1}{2} (x - \bar{x} - P_{XY}P_{YY}^{-1}(y - \bar{y}))^T (P_{XY}/P_{YY})^{-1} (x - \bar{x} - P_{XY}P_{YY}^{-1}(y - \bar{y}))\right) \\ &\quad \cdot \exp\left(-\frac{1}{2} (y - \bar{y})^T P_{YY}^{-1} (y - \bar{y})\right) \end{aligned}$$

From (2) it can be seen

$$\begin{aligned} (2\pi)^{(d_1+d_2)/2} |P_{XY}|^{1/2} &= (2\pi)^{(d_1+d_2)/2} (|P_{XY}/P_{YY}| |P_{YY}|)^{1/2} \\ &= (2\pi)^{d_1/2} |P_{XY}/P_{YY}|^{1/2} (2\pi)^{d_2/2} |P_{YY}|^{1/2} \end{aligned}$$

Hence

$$\begin{aligned} p(x, y | \hat{x}, P_{XY}) &= \frac{1}{(2\pi)^{d_1/2} |P_{XY}/P_{YY}|^{1/2}} \\ &\quad \cdot \exp\left(-\frac{1}{2} (x - \bar{x} - P_{XY}P_{YY}^{-1}(y - \bar{y}))^T (P_{XY}/P_{YY})^{-1} (x - \bar{x} - P_{XY}P_{YY}^{-1}(y - \bar{y}))\right) \\ &\quad \cdot \frac{1}{(2\pi)^{d_2/2} |P_{YY}|^{1/2}} \exp\left(-\frac{1}{2} (y - \bar{y})^T P_{YY}^{-1} (y - \bar{y})\right) \\ &= p(x|y) p(y) \end{aligned}$$

Therefore

$$\begin{aligned} p(x|y) &= \frac{1}{(2\pi)^{d_1/2} |P_{XY}/P_{YY}|^{1/2}} \\ &\quad \cdot \exp\left(-\frac{1}{2} (x - \bar{x} - P_{XY}P_{YY}^{-1}(y - \bar{y}))^T (P_{XY}/P_{YY})^{-1} (x - \bar{x} - P_{XY}P_{YY}^{-1}(y - \bar{y}))\right) \\ &\sim \mathcal{N}(\hat{x}, P_{XY}) \end{aligned}$$

where

$$\hat{x} = x + P_{XY}P_{YY}^{-1}(y - \bar{y})$$

$$P_{XY} = P_{XY}/P_{YY} = P_{XX} - P_{XY}P_{YY}^{-1}P_{YX}$$

2.5.ii)

⊙

i) Derive Kalman filter formula (2.52) and (2.53)

Specifically, show if $p(x_{t+1}|y_{0:t-1}) \sim \mathcal{N}(\hat{x}_{t+1|t-1}, P_{t+1|t-1})$
 then $p(x_t|y_{0:t-1}) \sim \mathcal{N}(\hat{x}_{t|t-1}, P_{t|t-1})$ where $\hat{x}_{t|t-1}$ and $P_{t|t-1}$
 are given by (2.52). Then using part i) show
 that $p(x_t|y_{0:t}) \sim \mathcal{N}(\hat{x}_{t|t}, P_{t|t})$ where $\hat{x}_{t|t}$ and $P_{t|t}$ are given by (2.53)

(2.52) Prediction:

$$\hat{x}_{t+1|t-1} = A_t \hat{x}_{t|t-1} \quad (2.52a)$$

$$P_{t+1|t-1} = A_t P_{t|t-1} A_t^T + W_t \quad (2.52b)$$

(2.53) Update:

$$\hat{x}_{t|t} = \hat{x}_{t|t-1} + P_{t|t-1} C_t^T (C_t P_{t|t-1} C_t^T + V_t)^{-1} (y_t - C_t \hat{x}_{t|t-1}) \quad (2.53a)$$

$$P_{t|t} = P_{t|t-1} - P_{t|t-1} C_t^T (C_t P_{t|t-1} C_t^T + V_t)^{-1} C_t P_{t|t-1} \quad (2.53b)$$

Show if $p(x_{t+1}|y_{0:t-1}) \sim \mathcal{N}(\hat{x}_{t+1|t-1}, P_{t+1|t-1})$

then $p(x_t|y_{0:t-1}) \sim \mathcal{N}(\hat{x}_{t|t-1}, P_{t|t-1})$ where $\hat{x}_{t|t-1}$ from (2.52a)

Linear model $x_{t+1} = A_t x_t + w_t$ so it is a linear transform
 $w_t \sim \mathcal{N}(0, W_t)$ $P_{t+1|t-1}$ from (2.52b)
 so $p(A_t x_{t+1|t-1}) \sim \mathcal{N}(A_t \hat{x}_{t+1|t-1}, A_t P_{t+1|t-1} A_t^T + W_t)$
 $\hat{x}_{t+1|t-1} = A_t \hat{x}_{t|t-1}$
 $\Rightarrow p(x_t|y_{0:t-1}) \sim \mathcal{N}(A_t \hat{x}_{t|t-1}, A_t P_{t|t-1} A_t^T + W_t)$ ← Gaussian adds for Gaussian

- ⊙ Now using part i) show that $p(x_t | y_{0:t}) \sim \mathcal{N}(\hat{x}_{t|t}, P_{t|t})$ where $\hat{x}_{t|t}$ & $P_{t|t}$ given by (2.53)

from i) $\hat{x} = \bar{x} + P_{xy} P_{yy}^{-1} (y - \bar{y})$

$$P_{xy} = P_{xy} / P_{yy} = P_{xx} - P_{xy} P_{yy}^{-1} P_{yx}$$

Want $\hat{x}_{t|t} = \hat{x}_{t|t-1} + P_{t|t-1} c_t^T (c_t P_{t|t-1} c_t^T + V_t)^{-1} (y_t - c_t \hat{x}_{t|t-1})$

directly \downarrow
 $p(x_t | y_{0:t}) \sim \mathcal{N}(\hat{x}_{t|t}, P_{t|t})$

$$P_{t|t} = P_{t|t-1} - \underbrace{P_{t|t-1} c_t^T}_{P_{xy}} \underbrace{(c_t P_{t|t-1} c_t^T + V_t)^{-1} c_t}_{P_{yy}^{-1}} \underbrace{P_{t|t-1} c_t}_{P_{yx}}$$

Expected value of y is $c_t \hat{x}_{t|t-1}$

because $y_t = c_t x_t + v_t, v_t \sim \mathcal{N}(0, V_t)$

$$\Rightarrow \mathbb{E}(y_t) = \mathbb{E}(c_t x_t) = c_t \mathbb{E}(x_t) = c_t \hat{x}_{t|t-1}$$

$$\mathbb{E}((y_t - c_t \hat{x}_{t|t-1})(y_t - c_t \hat{x}_{t|t-1})^T) = c_t P_{t|t-1} c_t^T + V_t$$

How to show $P_{yx} = c_t P_{t|t-1}$?

$$\begin{aligned} &= P_{yx} \\ &= \mathbb{E}((y_t - c_t \hat{x}_{t|t-1})(x_t - \hat{x}_{t|t-1})^T) \\ &= \mathbb{E}((c_t x_t - c_t \hat{x}_{t|t-1})(x_t - \hat{x}_{t|t-1})^T) \\ &= \mathbb{E}(c_t (x_t - \hat{x}_{t|t-1})(x_t - \hat{x}_{t|t-1})^T) \\ &= c_t \mathbb{E}((x_t - \hat{x}_{t|t-1})(x_t - \hat{x}_{t|t-1})^T) \\ &= c_t P_{t|t-1} \end{aligned}$$

KALMAN FILTER
DERIVED!!